src/LTS.v
@@ -72,7 +72,7 @@ Inductive step: St -> option Ev -> St -> Prop :=
 | statt:
     forall r lr x p q e req_loc rpy_loc,
       step (conf (aatt r lr (req_loc, rpy_loc) q x) p e)
-           (Some (req (fst r) req_loc p q (unanno x)))
+           (Some (req (fst r) req_loc p q (*(unanno x)*)))
            (rem (snd r) rpy_loc p (conf x q e))
 | stattstep:
     forall st0 ev st1 p j loc,
@@ -428,7 +428,7 @@ Proof.
     + exists (Some (asp_event (fst r) a n)).
       eapply ex_intro; eauto.
       
-    + exists (Some (req (fst r) (fst p) n n0 (unanno a))).
+    + exists (Some (req (fst r) (fst p) n n0 (*(unanno a)*))).
       repeat dest_range.
       eapply ex_intro; eauto.
     + exists None.
