src/Term_Defs.v
@@ -125,7 +125,7 @@ Inductive Ev: Set :=
 | umeas: nat -> Plc -> ASP_ID -> list Arg -> Ev
 | sign: nat -> Plc -> Ev
 | hash: nat -> Plc -> Ev
-| req: nat -> Loc -> Plc -> Plc -> Term -> Ev
+| req: nat -> Loc -> Plc -> Plc -> (*Term -> *) Ev
 | rpy: nat -> Loc -> Plc -> Plc -> Ev 
 (*| split: nat -> Plc -> Ev *)
 (*| splitp: nat -> (*Loc ->*) Loc -> Plc -> Ev *)
@@ -148,7 +148,7 @@ Definition ev x : nat :=
   | umeas i _ _ _  => i
   | sign i _ => i
   | hash i _ => i
-  | req i _ _ _ _ => i
+  | req i _ _ _ => i
   | rpy i _ _ _ => i 
   (*| split i _ => i *)
   (* | splitp i _ _ => i *)
@@ -163,7 +163,7 @@ Definition pl x : Loc :=
   | umeas _ p _ _  => p
   | sign _ p => p
   | hash _ p => p
-  | req _ _ p _ _ => p
+  | req _ _ p _ => p
   | rpy _ _ p _ => p
   (*| split _ p => p *)
   (*| splitp _ _ p => p *)
